Stratego/JavaExport.thy
@@ -1,0 +1,285 @@
+theory JavaExport
+  imports CompileRewrite
+begin
+
+class JavaStatement =
+  fixes statementToJava :: "nat \<Rightarrow> 'a \<Rightarrow> string"
+
+class JavaExpression =
+  fixes expToJava :: "'a \<Rightarrow> string"
+
+type_synonym ClassName = string
+type_synonym VariableName = string
+type_synonym MethodName = string
+
+datatype 'a BaseExpressions =
+  Ref VariableName |
+  IntegerConstant int |
+  TrueValue |
+  FalseValue |
+  MethodCall "'a::JavaExpression" MethodName "'a::JavaExpression list" |
+  Constructor ClassName "'a::JavaExpression list" |
+  InstanceOf "'a BaseExpressions" ClassName VariableName |
+  Equal "'a BaseExpressions" "'a BaseExpressions" |
+  ConditionExpression 'a (* |
+  Less Expression Expression |
+  Negate Expression |
+  And Expression Expression |
+  BitAnd Expression Expression |
+  Unsupported string*)
+
+datatype ('a) Statement =
+  Assignment VariableName "'a::JavaExpression" |
+  Branch "'a::JavaExpression" "('a) Statement" |
+  Return "'a::JavaExpression" |
+  Sequential "('a) Statement list"
+
+fun intersperse :: "string \<Rightarrow> string list \<Rightarrow> string list" where
+  "intersperse i es = foldr (\<lambda>x ys . x # (if ys = [] then ys else i # ys)) es []"
+
+fun param_list :: "string list \<Rightarrow> string" where
+  "param_list es = (foldr (@) (intersperse '', '' es) '''')"
+
+fun generate_expression :: "('a::JavaExpression) BaseExpressions \<Rightarrow> string" where
+  "generate_expression (Ref v) = v" |
+  "generate_expression (IntegerConstant n) = ''0''" | (*TODO FIX*)
+  "generate_expression TrueValue = ''true''" |
+  "generate_expression FalseValue = ''false''" |
+  "generate_expression (MethodCall e mn ps) = 
+    (expToJava e) @ ''.'' @ mn @ ''('' @ param_list (map expToJava ps) @ '')''" |
+  "generate_expression (Constructor cn ps) =
+    ''new '' @ cn @ ''('' @ param_list (map expToJava ps) @ '')''" |
+  "generate_expression (InstanceOf e cn v) =
+    (generate_expression e) @ '' instanceof '' @ cn @ '' '' @ v" |
+  "generate_expression (Equal e1 e2) =
+    (generate_expression e1) @ '' == '' @ (generate_expression e2)" |
+  "generate_expression (ConditionExpression e) =
+    (expToJava e)"
+
+fun indent :: "nat \<Rightarrow> string" where
+  "indent 0 = ''''" |
+  "indent (Suc n) = '' '' @ indent n"
+
+fun generate_statement :: "nat \<Rightarrow> ('a::JavaExpression) Statement \<Rightarrow> string" where
+  "generate_statement i (Assignment v e) = indent i @
+    ''var '' @ v @ '' = '' @ expToJava e @ '';\<newline>''" |
+  "generate_statement i (Branch c s) = indent i @
+    ''if ('' @ expToJava c @ '') {\<newline>'' @ generate_statement (i + 4) s @ 
+    indent i @ ''}\<newline>''" |
+  "generate_statement i (Return e) = indent i @
+    ''return '' @ expToJava e @ '';\<newline>''" |
+  "generate_statement i (Sequential ss) = 
+    foldr (@) (map (generate_statement i) ss) ''''"
+
+
+instantiation "BaseExpressions" :: (type) JavaExpression
+begin
+definition "expToJava_BaseExpressions = generate_expression" 
+instance ..
+end
+
+instantiation "Statement" :: (type) JavaStatement
+begin
+definition "statementToJava_Statement = generate_statement" 
+instance ..
+end
+ 
+
+locale JavaTarget = CompiledRewrites +
+  fixes class_of_term :: "'a \<Rightarrow> string"
+  and generate_condition :: "'b \<Rightarrow> 'e::JavaExpression"
+  and generate_result :: "'c \<Rightarrow> 'e::JavaExpression"
+  and generate_access :: "VarName \<Rightarrow> 'a \<Rightarrow> 'e::JavaExpression list"
+  (*and generate_assignment :: "VarName \<Rightarrow> 'a \<Rightarrow> ('e BaseExpressions) Statement \<Rightarrow> ('e BaseExpressions) Statement"*)
+begin
+
+fun generate_assignment :: 
+  "VarName \<Rightarrow> 'a \<Rightarrow> ('e BaseExpressions) Statement \<Rightarrow> ('e BaseExpressions) Statement" where
+  "generate_assignment v e s =
+    Sequential (
+      [Assignment e' (ConditionExpression ((generate_access (v @ ''c'') e)!i)).
+        (i, e') <- (enumerate 0 (pattern_variables e))] @ [s])"
+
+function (sequential) export_match :: "('a, 'b) MATCH \<Rightarrow> ('e BaseExpressions) Statement 
+  \<Rightarrow> ('e BaseExpressions) Statement" where
+  "export_match (match v p) r  = 
+    Branch (InstanceOf (Ref v) (class_of_term p) (v @ ''c''))
+      (Sequential [(generate_assignment v p r)])" |
+  "export_match (andthen m1 m2) r = 
+    export_match m1 (export_match m2 r)" |
+  "export_match (equality v1 v2) r = 
+    Branch (Equal (Ref v1) (Ref v2)) r" |
+  "export_match (cond sc) r = 
+    Branch (ConditionExpression (generate_condition sc)) r" |
+  "export_match noop r = r"
+  apply pat_completeness+
+  by simp+
+
+fun size_conditional :: "(('a, 'b) MATCH \<times> ('e BaseExpressions) Statement) \<Rightarrow> nat" where
+  "size_conditional ((cond c), s) = size_match (cond c) + size_condition c" |
+  "size_conditional (m, s) = size_match m"
+
+termination export_match
+  apply (relation "measures [size_conditional]") apply simp apply simp sorry
+
+
+fun export_rules :: "('a, 'b, 'c) Rules \<Rightarrow> ('e BaseExpressions) Statement" where
+  "export_rules (base e) = Return (ConditionExpression (generate_result e))" |
+  "export_rules (cond' m r) = export_match m (export_rules r)" |
+  "export_rules (r1 else r2) = Sequential [export_rules r1, export_rules r2]" |
+  "export_rules (choice rules) = Sequential (map export_rules rules)" |
+  "export_rules (r1 \<then> r2) = Sequential [export_rules r1, export_rules r2]" (* TODO: should modify e *)
+end
+
+
+
+
+fun class_of_term_Arithmetic :: "Arithmetic \<Rightarrow> string" where
+  "class_of_term_Arithmetic (Add x y) = ''AddNode''" |
+  "class_of_term_Arithmetic (Sub x y) = ''SubNode''" |
+  "class_of_term_Arithmetic (UMinus x) = ''UnaryMinusNode''" |
+  "class_of_term_Arithmetic (Number v) = ''ConstantNode''" |
+  "class_of_term_Arithmetic (Variable s) = ''VariableNode''"
+
+datatype JavaCheck =
+  CallMethod1 |
+  CallMethod2 |
+  MethodCall string string |
+  Construct string "JavaCheck list" |
+  VariableExpr string
+
+instantiation "JavaCheck" :: JavaExpression
+begin
+fun expToJava_JavaCheck where
+  "expToJava_JavaCheck CallMethod1 = ''I'm asserting you're a number''" |
+  "expToJava_JavaCheck CallMethod2 = ''I'm asserting you're a subnode''" |
+  "expToJava_JavaCheck (MethodCall ob m) = ob @ ''.'' @ m @ ''()''" |
+  "expToJava_JavaCheck (Construct class args) = ''new '' @ class @ ''('' @ param_list (map expToJava_JavaCheck args) @ '')''" |
+  "expToJava_JavaCheck (VariableExpr v) = v"
+instance ..
+end
+
+fun generate_condition_Arithmetic :: "ArithmeticCondition \<Rightarrow> JavaCheck" where
+  "generate_condition_Arithmetic (IsSub e) = CallMethod2" |
+  "generate_condition_Arithmetic (IsNumber e) = CallMethod1"
+
+fun generate_Arithmetic :: "Arithmetic \<Rightarrow> JavaCheck" where
+  "generate_Arithmetic (Add x y) = Construct ''AddNode'' (map generate_Arithmetic [x, y])" |
+  "generate_Arithmetic (Sub x y) = Construct ''SubNode'' (map generate_Arithmetic [x, y])" |
+  "generate_Arithmetic (UMinus x) = Construct ''UnaryMinusNode'' (map generate_Arithmetic [x])" |
+  "generate_Arithmetic (Number v) = Construct ''ConstantNode'' []" |
+  "generate_Arithmetic (Variable s) = VariableExpr s"
+
+fun generate_result_Arithmetic :: "Transformer \<Rightarrow> JavaCheck" where
+  "generate_result_Arithmetic (UnaryMinus e) = CallMethod1" |
+  "generate_result_Arithmetic (Plus e1 e2) = CallMethod2" |
+  "generate_result_Arithmetic (Result e) = generate_Arithmetic e"
+
+fun generate_access_Arithmetic :: "VarName \<Rightarrow> Arithmetic \<Rightarrow> JavaCheck list" where
+  "generate_access_Arithmetic v (Add x y) = 
+    [(MethodCall v ''getX''),
+     (MethodCall v ''getY'')]" |
+  "generate_access_Arithmetic v (Sub x y) = 
+    [(MethodCall v ''getX''),
+     (MethodCall v ''getY'')]" |
+  "generate_access_Arithmetic v (UMinus x) = [(MethodCall v ''getValue'')]" |
+  "generate_access_Arithmetic v (Number val) = []" |
+  "generate_access_Arithmetic v (Variable s) = []"
+
+(*
+  "export_assignments v (UnaryPattern op v1) s = Sequential
+    [Assignment v1 (MethodCall (Ref (v + STR ''c'')) ''getValue'' []), s]" |
+  "export_assignments v (BinaryPattern op v1 v2) s = Sequential
+    [Assignment v1 (MethodCall (Ref (v + STR ''c'')) ''getX'' []),
+     Assignment v2 (MethodCall (Ref (v + STR ''c'')) ''getY'' []), s]" |
+  "export_assignments v (ConditionalPattern v1 v2 v3) s = Sequential
+    [Assignment v1 (MethodCall (Ref (v + STR ''c'')) ''condition'' []),
+     Assignment v2 (MethodCall (Ref (v + STR ''c'')) ''trueValue'' []),
+     Assignment v3 (MethodCall (Ref (v + STR ''c'')) ''falseValue'' []), s]" |
+  "export_assignments v (ConstantPattern val) s =
+    Branch (InstanceOf (MethodCall (Ref (v + STR ''c'')) ''getValue'' []) ''PrimitiveConstant'' (v + STR ''cd''))
+    (Branch (Equal (MethodCall (Ref (v + STR ''cd'')) ''asLong'' []) (export_value val)) s)" |
+  "export_assignments v (ConstantVarPattern var) s =
+    Branch (Equal (MethodCall (Ref (v + STR ''c'')) ''getValue'' []) (Ref var)) s" |
+  "export_assignments v (VariablePattern var) s =
+    Return (Unsupported ''export_assignments for VariablePattern'')" 
+*)
+
+setup \<open>Locale_Code.open_block\<close>
+interpretation Arithmetic: JavaTarget
+  size_Arithmetic
+  "eval_condition"
+  "ground_condition"
+  "is_ground_condition"
+  "eval_transformer"
+  "ground_transformer"
+  "is_ground_transformer"
+  rewrite_Arithmetic
+  match_Arithmetic
+  varof_Arithmetic
+  var_Arithmetic
+  subexprs_Arithmetic
+  chain_Arithmetic
+  class_of_term_Arithmetic
+  generate_condition_Arithmetic
+  generate_result_Arithmetic
+  generate_access_Arithmetic
+proof
+  fix e :: Arithmetic
+  show "\<forall>e' \<in> set (subexprs_Arithmetic e). size_Arithmetic e > size_Arithmetic e'"
+    by (cases e; simp)
+next
+  fix f :: "Arithmetic \<Rightarrow> Arithmetic"
+  fix e :: Arithmetic
+  show "map f (subexprs_Arithmetic e) = subexprs_Arithmetic (snd (chain_Arithmetic (\<lambda>e a. (plus a 1, f e)) e 0))"
+    by (cases e; simp)
+next
+  fix f :: "Arithmetic \<Rightarrow> Arithmetic"
+  fix e :: Arithmetic
+  show "length (subexprs_Arithmetic e) = fst (chain_Arithmetic (\<lambda>e a. (plus a 1, f e)) e 0)"
+    by (cases e; simp)
+qed
+setup \<open>Locale_Code.close_block\<close>
+
+definition "export_rules = Arithmetic.export_rules"
+
+
+value "export_rules"
+
+definition "join = Arithmetic.join"
+(*definition "compile' = ArithmeticCompiled.compile'"*)
+definition "generate = Arithmetic.generate"
+definition "match_pattern = Arithmetic.match_pattern"
+definition "optimized_export = Arithmetic.optimized_export"
+
+export_code "optimized_export" checking SML
+
+definition Identity where
+  "Identity = generate 
+    (Add
+      (var ''x'')
+      (Number 0))
+    (Result (var ''x''))"
+
+value "Identity"
+text "@{value[display] \<open>Identity\<close>}"
+value "optimized_export Identity"
+text "@{value[display] \<open>optimized_export Identity\<close>}"
+
+text \<open>@{text "const x + const y \<longrightarrow> const (x + y)"}\<close>
+definition Evaluate where
+  "Evaluate = generate 
+    (Add
+      (var ''x'')
+      (var ''y''))
+    (Plus (var ''x'') (var ''y''))"
+(* doesn't support constant evaluation *)
+value "Evaluate"
+value "(optimized_export (Evaluate))"
+
+
+value "export_rules (optimized_export (choice [Identity, Evaluate]))"
+
+value "statementToJava 0 (export_rules (optimized_export (choice [Identity, Evaluate])))"
+
+end
